merge with distance_fix

src/Core/PtrLemmas.v
@@ -1,19 +1,23 @@
-Require Import Core Notations.
 Require Import StructTact.StructTactics.
+Require Import Core Notations Tactics.
 
-(* Address [b,ofs] *)
+(* Address: [b,ofs] *)
 Definition addr : Type := (block * ptrofs).
-Definition vptr (a : addr) := match a with (b,ofs) => Vptr b ofs end.
+Definition vptr (a : addr) := match a with (b, ofs) => Vptr b ofs end.
 Definition load_addr (chunk : memory_chunk) (m : mem) (a : addr) :=
   match a with (b,ofs) => Mem.loadv chunk m (Vptr b ofs) end.
-Definition next_addr (a : addr) := match a with (b,ofs) => (b, Ptrofs.add ofs Ptrofs.one) end.
-Definition add_addr (a : addr) (i : ptrofs) := match a with (b,ofs) => (b, Ptrofs.add ofs i) end.
+Definition next_addr (a : addr) := match a with 
+                                     (b, ofs) => (b, Ptrofs.add ofs Ptrofs.one) 
+                                   end.
+Definition add_addr (a : addr) (i : ptrofs) := 
+  match a with (b, ofs) => (b, Ptrofs.add ofs i) end.
 Notation "a ++" := (next_addr a) (at level 20).
 
 (* Pointer comparison *)
 (* Abstract spec : [b1,ofs1] >= [b2,ofs2] *)
 Definition ptr_ge_spec (b1 b2 : block) (ofs1 ofs2 : ptrofs) :=
   if eq_block b1 b2 then Some (ofs2 <=u ofs1)%ptrofs else None.
+
 (* Spec using Compcert semantic values *)
 Definition ptr_ge (m : mem) (b1 b2 : block) (ofs1 ofs2 : ptrofs) :=
   if Archi.ptr64
@@ -23,7 +27,8 @@ Definition ptr_ge (m : mem) (b1 b2 : block) (ofs1 ofs2 : ptrofs) :=
 Definition addr_ge (m : mem) (a1 a2 : addr) :=
   match a1, a2 with (b1, ofs1), (b2, ofs2) => ptr_ge m b1 b2 ofs1 ofs2 end.
 
-Definition addr_lt (m : mem) (a1 a2 : addr) := option_map negb (addr_ge m a2 a1).
+Definition addr_lt (m : mem) (a1 a2 : addr) := 
+  option_map negb (addr_ge m a2 a1).
 
 (* Both specs can be used interchangeably *)
 Proposition ptr_ge_refine : forall (m : mem) (b1 b2 : block) (ofs1 ofs2 : ptrofs),
@@ -37,12 +42,14 @@ Proof.
   destruct Archi.ptr64 eqn: A; simpl.
   all: rewrite H; rewrite H0; simpl;
     destruct (Mem.valid_pointer m b1 (Ptrofs.unsigned ofs1) &&
-                                Mem.valid_pointer m b2 (Ptrofs.unsigned ofs2)); auto.
+                                Mem.valid_pointer m b2 (Ptrofs.unsigned ofs2));
+    auto.
 Qed.
 
 Proposition ptr_ge_to_sem_cmp_true : forall m b1 b2 i1 i2,
     ptr_ge m b1 b2 i1 i2 = Some true ->
-    sem_cmp Cge (Vptr b1 i1) (tptr tschar) (Vptr b2 i2) (tptr tschar) m = Some Vtrue.
+    sem_cmp Cge (Vptr b1 i1) (tptr tschar) (Vptr b2 i2) (tptr tschar) m = 
+    Some Vtrue.
 Proof.
   intros.
   assert ((option_map Val.of_bool (ptr_ge m b1 b2 i1 i2)) =
@@ -52,7 +59,8 @@ Qed.
 
 Proposition ptr_ge_to_sem_cmp_false : forall m b1 b2 i1 i2,
     ptr_ge m b1 b2 i1 i2 = Some false ->
-    sem_cmp Cge (Vptr b1 i1) (tptr tschar) (Vptr b2 i2) (tptr tschar) m = Some Vfalse.
+    sem_cmp Cge (Vptr b1 i1) (tptr tschar) (Vptr b2 i2) (tptr tschar) m = 
+    Some Vfalse.
 Proof.
   intros.
   assert ((option_map Val.of_bool (ptr_ge m b1 b2 i1 i2)) =
@@ -61,57 +69,93 @@ Proof.
 Qed.
 
 (* distance between addresses *)
-Definition distance (a1 a2 : addr) : nat :=
-  ((Z.to_nat (Ptrofs.unsigned (snd a2))) - (Z.to_nat (Ptrofs.unsigned (snd a1))))%nat.
+Definition distance (m : mem) (a1 a2 : addr) : option nat :=
+  match addr_ge m a2 a1 with
+  | Some true => Some ((Z.to_nat (Ptrofs.unsigned (snd a2))) -
+                      (Z.to_nat (Ptrofs.unsigned (snd a1))))%nat
+  | _ => None
+  end.
 
-Lemma dist_succ : forall b b' ofs ofs' dist,
-    distance (b', ofs') (b, ofs) = S dist ->
-    distance (b', (Ptrofs.add ofs' Ptrofs.one)) (b, ofs) = dist.
+Lemma dist_succ : forall m b b' ofs ofs' dist,
+    distance m (b', ofs') (b, ofs) = Some (S dist) ->
+    Mem.valid_pointer m b' (Ptrofs.unsigned (ofs' + 1)%ptrofs) = true ->
+    distance m (b', (Ptrofs.add ofs' Ptrofs.one)) (b, ofs) = Some dist.
 Proof.
-  intros b b' ofs ofs' dist Dist.
-  unfold distance, snd.
-  rewrite <-Z2Nat.inj_sub by (apply Ptrofs.unsigned_range).
-  assert ((distance (b', ofs') (b, ofs) = S dist) 
-          <-> 
-          ((distance (b', ofs') (b, ofs) - 1)%nat = dist)) by lia.
-  unfold distance, snd in Dist.
-  assert ( (Ptrofs.unsigned ofs') < (Ptrofs.unsigned ofs))%Z.
-  {
-    assert ((Z.to_nat (Ptrofs.unsigned ofs') 
-             < 
-             Z.to_nat (Ptrofs.unsigned ofs))%nat) by lia.
-    unfold Ptrofs.unsigned in *.
-    destruct ofs, ofs'; simpl in *.
-    pose proof (Z2Nat.inj_lt intval0 intval) as Inj.
-    destruct Inj.
-    all: try lia.
-  }
-  rewrite H in Dist.
-  unfold distance, snd in Dist.
-  rewrite <-Z2Nat.inj_sub in Dist by (apply Ptrofs.unsigned_range).
-  rewrite <-Dist.
-  replace ((1)%nat) with ((Z.to_nat (1)%Z)) by reflexivity.
-  rewrite <-Z2Nat.inj_sub; [| lia].
-  f_equal.
-  assert (Ptrofs.unsigned (Ptrofs.add ofs' Ptrofs.one) 
-          = (Ptrofs.unsigned ofs' + 1)%Z); [|lia].
-  replace (1%Z) with (Ptrofs.unsigned Ptrofs.one) by reflexivity.
-  rewrite Ptrofs.add_unsigned.
+  unfold distance, snd; intros.
+  break_match_hyp; [| discriminate].
+  break_if; subst; [| discriminate].
+  inversion H; clear H.
   assert (Ptrofs.unsigned ofs' < Ptrofs.max_unsigned)%Z.
   {
+    assert ((Ptrofs.unsigned ofs') < (Ptrofs.unsigned ofs))%Z.
+    {
+      assert ((Z.to_nat (Ptrofs.unsigned ofs') 
+               < 
+               Z.to_nat (Ptrofs.unsigned ofs))%nat) by lia.
+      unfold Ptrofs.unsigned in *.
+      destruct ofs, ofs'; simpl in *.
+      pose proof (Z2Nat.inj_lt intval0 intval) as Inj.
+      destruct Inj.
+      all: try lia.
+    }
     assert (Ptrofs.unsigned ofs <= Ptrofs.max_unsigned)%Z.
     pose proof (Ptrofs.unsigned_range_2 ofs).
     all: try lia.
   }
-  rewrite Ptrofs.unsigned_repr.
+  replace (addr_ge m (b, ofs) (b', (ofs' + 1)%ptrofs))
+    with (Some true).
+  f_equal.
+  enough (S (Z.to_nat (Ptrofs.unsigned (ofs')%ptrofs)) =
+             Z.to_nat (Ptrofs.unsigned (ofs' + 1)%ptrofs)) by lia.
+  rewrite Ptrofs.add_unsigned, Ptrofs.unsigned_repr, <-Z2Nat.inj_succ.
   reflexivity.
-  pose proof Ptrofs.unsigned_range ofs.
-  assert (Ptrofs.unsigned ofs' + 1 <= Ptrofs.max_unsigned)%Z by lia.
-  replace (Ptrofs.unsigned Ptrofs.one)%Z with (1)%Z by reflexivity.
-  assert (0 <= Ptrofs.unsigned ofs')%Z 
-    by (apply Ptrofs.unsigned_range).
+  apply Ptrofs.unsigned_range.
+  replace (Ptrofs.unsigned 1%ptrofs) with 1 by reflexivity.
+  pose proof Ptrofs.unsigned_range ofs'.
   lia.
+
+  unfold addr_ge, ptr_ge in *.
+  simpl in *.
+  repeat break_if; subst.
+  all: try discriminate.
+  all: repeat destruct_andb_hyp.
+  all: repeat destruct_orb_hyp.
+  all: try congruence.
+  all: clear - H H2 Heqo.
+
+  all: assert (Z.to_nat (Ptrofs.unsigned ofs') + 1 <=
+          Z.to_nat (Ptrofs.unsigned ofs))%nat
+    by lia.
+  all: unfold Ptrofs.ltu.
+  all: break_if.
+  all: rewrite Ptrofs.add_unsigned, Ptrofs.unsigned_repr in *.
+  all: replace (Ptrofs.unsigned 1%ptrofs) with 1 in * by reflexivity.
+  all: replace (1)%nat with (Z.to_nat 1)%nat in H0 by reflexivity.
+  all: rewrite <-Z2Nat.inj_add in H0.
+  all: try rewrite <-Z2Nat.inj_le in H0.
+  all: try apply Ptrofs.unsigned_range.
+  all: try reflexivity.
+  all: replace (Ptrofs.unsigned 1%ptrofs) with 1 by reflexivity.
+  all: pose proof Ptrofs.unsigned_range ofs'.
+  all: try lia.
 Qed.
+
+Lemma dist_to_lt : forall m b ofs ofs' dist, 
+  distance m (b, ofs) (b, ofs') = Some (S dist) ->
+  (Ptrofs.unsigned ofs < Ptrofs.unsigned ofs')%Z.
+Proof.
+  intros;
+  unfold distance in *; simpl in *.
+  break_match_hyp; [| discriminate].
+  break_if; [| discriminate].
+  inversion H; clear H; rename H1 into H.
+  assert ((Z.to_nat (Ptrofs.unsigned ofs) 
+             < 
+             Z.to_nat (Ptrofs.unsigned ofs'))%nat) by lia.
+  unfold Ptrofs.unsigned in *.
+  destruct ofs, ofs'; simpl in *.
+  apply Z2Nat.inj_lt; lia.
+Qed.  
 
 Lemma if_some (c x : bool) :
     (if c then Some x else None) = Some false ->
@@ -128,72 +172,29 @@ Proof.
 Qed.
 
 Lemma dist_pred: 
-  forall (m : mem) (str_b : block) (str_ofs : ptrofs) (b : block) (i : ptrofs), 
-    addr_ge m (str_b, str_ofs) (b, i) = Some false -> 
-    addr_ge m ((str_b, str_ofs) ++) (b, i) = Some false -> 
-    (distance (str_b, str_ofs) (b, i) - 1)%nat = 
-    distance (str_b, (str_ofs + 1)%ptrofs) (b, i).
-Proof.
-  intros m str_b str_ofs b i Heqo0 Heqo2.
-  remember (distance (str_b, str_ofs) (b, i) - 1)%nat as
-      dist.
-  symmetry.
-  apply dist_succ.
-  rewrite Heqdist.
-  unfold distance; simpl.
-  rewrite <-Nat.add_1_l.
-  repeat replace 1%nat with (Z.to_nat 1)%Z by reflexivity.
-  repeat rewrite <-Z2Nat.inj_sub;
-    [| lia | apply Ptrofs.unsigned_range].
-  rewrite <-Z2Nat.inj_add; [| lia |].
-  f_equal; lia.
-  unfold addr_ge, ptr_ge in Heqo2, Heqo0.
-  simpl in Heqo2, Heqo0.
-  destruct Archi.ptr64 in Heqo2, Heqo0.
-  all: destruct eq_block in Heqo2, Heqo0.
-  1,3: apply if_some in Heqo0.
-  1,2: rewrite negb_false_iff in Heqo0.
-  1,2: apply Ptrofs.ltu_inv in Heqo0.
-  1,2: lia.
-  all: apply if_none in Heqo2.
-  all: discriminate.
-Qed.
-
-Lemma dist_to_lt : forall b b' ofs ofs' dist, 
-  distance (b', ofs') (b, ofs) = S dist ->
-  (Ptrofs.unsigned ofs' < Ptrofs.unsigned ofs)%Z.
-Proof.
-  intros;
-  unfold distance in *; simpl in *.
-  assert ((Z.to_nat (Ptrofs.unsigned ofs') 
-             < 
-             Z.to_nat (Ptrofs.unsigned ofs))%nat) by lia.
-  unfold Ptrofs.unsigned in *.
-  destruct ofs, ofs'; simpl in *.
-  pose proof (Z2Nat.inj_lt intval0 intval) as Inj.
-  destruct Inj.
-  all: try lia.
-Qed.  
-  
-Lemma dist_to_lt_or_ge : forall b b' ofs ofs' dist, 
-    distance (b', ofs') (b, ofs) = dist ->
-    (Ptrofs.unsigned ofs' <= Ptrofs.unsigned ofs)%Z.
-Proof.
-  destruct dist; intros.
-  - unfold distance in *; simpl in *.
-    assert ((Z.to_nat (Ptrofs.unsigned ofs) <= 
-             Z.to_nat (Ptrofs.unsigned ofs'))%nat) by lia.
-    unfold Ptrofs.unsigned in *.
-    destruct ofs, ofs'; simpl in *.
-    pose proof (Z2Nat.inj_le intval0 intval) as Inj.
-    destruct Inj.
-    all: try lia.
-    eapply H2.
-Admitted.
+  forall (m : mem) (b : block) (ofs : ptrofs) (i : ptrofs) (dist : nat), 
+    addr_ge m (b, ofs) (b, i) = Some false -> 
+    addr_ge m ((b, ofs) ++) (b, i) = Some false -> 
+    distance m (b, ofs) (b, i) = Some (dist - 1)%nat ->
+    Mem.valid_pointer m b (Ptrofs.unsigned (ofs + 1)%ptrofs) = true ->
+    distance m (b, (ofs + 1)%ptrofs) (b, i) = Some dist.
+  Admitted.
 
 Lemma int_ptrofs_mod_eq : (Int.modulus = Ptrofs.modulus).
 Proof.
   reflexivity.
+Qed.
+
+Lemma loaded_is_valid : forall c m b ofs v,
+  Mem.load c m b ofs = Some v ->
+  Mem.valid_pointer m b ofs = true.
+Proof.
+  intros.
+  apply Mem.valid_pointer_nonempty_perm.
+  apply Mem.load_valid_access in H.
+  apply Mem.valid_access_perm with (k := Cur) in H.
+  apply Mem.perm_implies with (p2 := Nonempty) in H; [| constructor].
+  assumption.
 Qed.
 
 Hint Resolve Ptrofs.mul_one Ptrofs.add_zero int_ptrofs_mod_eq : ptrofs.
